

# Homework 1

● Graded

Student

Nick Zhu

Total Points

100 / 100 pts

Question 1

Problem 1

20 / 20 pts

✓ - 0 pts Correct

Question 2

Problem 2

30 / 30 pts

2.1 (a)

10 / 10 pts

✓ - 0 pts Correct

2.2 (b)

10 / 10 pts

✓ - 0 pts Correct

2.3 (c)

10 / 10 pts

✓ - 0 pts Correct

Question 3

Problem 3

20 / 20 pts

3.1 (a)

15 / 15 pts

✓ - 0 pts Correct

3.2 (b)

5 / 5 pts

✓ - 0 pts Correct

Question 4

Problem 4

30 / 30 pts

4.1 (a)

6 / 6 pts

✓ - 0 pts Correct

4.2 (b)

12 / 12 pts

✓ - 0 pts Correct

4.3 (c)

12 / 12 pts

✓ - 0 pts Correct

Question assigned to the following page: [1](#)

Problem 1 (20 pts)

Put the following functions in order in terms of  $o$ -notation:

1.  $\sqrt{n}$
2.  $2^{\log_3 n}$
3.  $(\log n)^2$
4.  $3^n$
5.  $n^3$
6.  $8^{n/2}$

Prove that your relation is correct for each adjacent pair. In particular, if your functions are ordered as  $f_1, f_2, f_3, f_4, f_5, f_6$ ; then show that  $f_1 \in o(f_2)$  and  $f_2 \in o(f_3)$  and so on.

## Solution

### Step 1. Ordering

The functions ordered from slowest to fastest growth are as follows:

$$(\log n)^2, \quad \sqrt{n}, \quad 2^{\log_3 n}, \quad n^3, \quad 8^{n/2}, \quad 3^n$$

In  $o$ -notation, we write

$$(\log n)^2 \in o(\sqrt{n}) \in o(2^{\log_3 n}) \in o(n^3) \in o(8^{n/2}) \in o(3^n).$$

### Step 2. Simplification

Before proving the relations, we simplify the functions to make the proofs easier.

Using the identity

$$a^{\log_b n} = n^{\log_b a}$$

we have

$$2^{\log_3 n} = n^{\log_3 2} \approx n^{0.63}$$

Also,

$$8^{n/2} = (8^{1/2})^n = (2\sqrt{2})^n$$

### Step 3. Proofs

- 1.  $(\log n)^2 \in o(\sqrt{n})$ : We need to show that

$$\lim_{n \rightarrow \infty} \frac{(\log n)^2}{\sqrt{n}} = 0.$$

Let  $n = 2^m$ . Then,

$$\log n = m \quad \text{and} \quad \sqrt{n} = 2^{m/2}.$$

Question assigned to the following page: [1](#)

Thus,

$$\frac{(\log n)^2}{\sqrt{n}} = \frac{m^2}{2^{m/2}},$$

and as  $m \rightarrow \infty$ , the exponential term in the denominator dominates the polynomial numerator, so the limit is 0.

- 2.  $\sqrt{n} \in o(2^{\log_3 n})$ : Since  $2^{\log_3 n} = n^{\log_3 2}$ , we have

$$\frac{\sqrt{n}}{2^{\log_3 n}} = \frac{n^{1/2}}{n^{\log_3 2}} = n^{1/2 - \log_3 2}.$$

Because  $1/2 - \log_3 2 < 0$ ,

$$\lim_{n \rightarrow \infty} n^{1/2 - \log_3 2} = 0.$$

- 3.  $2^{\log_3 n} \in o(n^3)$ : Since  $2^{\log_3 n} = n^{\log_3 2}$ , we have

$$\frac{2^{\log_3 n}}{n^3} = \frac{n^{\log_3 2}}{n^3} = n^{\log_3 2 - 3}.$$

Because  $\log_3 2 - 3 < 0$ ,

$$\lim_{n \rightarrow \infty} n^{\log_3 2 - 3} = 0.$$

- 4.  $n^3 \in o(8^{n/2})$ : Since the exponential function  $8^{n/2}$  grows much faster than the polynomial  $n^3$ , we have

$$\lim_{n \rightarrow \infty} \frac{n^3}{8^{n/2}} = 0,$$

- 5.  $8^{n/2} \in o(3^n)$ : We have

$$\frac{8^{n/2}}{3^n} = \left(\frac{8^{1/2}}{3}\right)^n = \left(\frac{2\sqrt{2}}{3}\right)^n.$$

Since  $\frac{2\sqrt{2}}{3} < 1$ ,

$$\lim_{n \rightarrow \infty} \left(\frac{2\sqrt{2}}{3}\right)^n = 0.$$

Questions assigned to the following page: [2.1](#), [2.2](#), and [2.3](#)

Problem 2 (30 pts)

Consider the function  $f(n) = n \cdot (n \bmod 2) + \log n$ .

- (a) Show that  $f(n) \in O(n)$  and  $f(n) \in \Omega(\log n)$ .
- (b) Show that neither  $f(n) \in \Theta(n)$  nor  $f(n) \in \Theta(\log n)$ .
- (c) Suppose for some function  $g(n)$ , we have  $f(n) \notin O(g(n))$ . Is it always true that  $f(n) \in \omega(g(n))$ ? Justify your answer with either a proof or a counter-example.

**Solution**

(a)

$f(n) \in O(n)$ : For any  $n \geq 2$ :

$$\begin{aligned} \text{If } n \text{ is even: } f(n) &= \log n \leq n, \\ \text{If } n \text{ is odd: } f(n) &= n + \log n \leq n + n = 2n. \end{aligned}$$

Thus,  $f(n) \leq 2n$  for all  $n \geq 2$ . Choosing  $C = 2$  and  $n_0 = 2$  gives  $f(n) \in O(n)$ .

$f(n) \in \Omega(\log n)$ : For all  $n$ :

$$\begin{aligned} \text{If } n \text{ is even: } f(n) &= \log n, \\ \text{If } n \text{ is odd: } f(n) &= n + \log n \geq \log n. \end{aligned}$$

Thus, let  $c = 1$  we have  $f(n) \geq \log n$  for all  $n$ , so  $f(n) \in \Omega(\log n)$ .

(b)

We prove by contradiction.

Assume  $f(n) \in \Theta(n)$ , then there exist constants  $c_1, c_2 > 0$  and  $n_0$  such that for all  $n \geq n_0$ ,

$$c_1 n \leq f(n) \leq c_2 n.$$

However, when  $n$  is even,  $f(n) = \log n$  and the inequality  $c_1 n \leq \log n$  fails for large  $n$  (since  $\log n/n \rightarrow 0$ ). Thus, we've reached a contradiction and  $f(n) \notin \Theta(n)$ .

Similarly, assume  $f(n) \in \Theta(\log n)$ , then there exist constants  $c_1, c_2 > 0$  such that for all large  $n$ ,

$$c_1 \log n \leq f(n) \leq c_2 \log n.$$

But for odd  $n$ ,  $f(n) = n + \log n$  grows like  $n$ , which is much larger than any constant multiple of  $\log n$ . Thus, we've reached a contradiction and  $f(n) \notin \Theta(\log n)$ .

(c)

It is not always true. We will show a counterexample.

Counterexample: Define

$$g(n) = \begin{cases} n, & \text{if } n \text{ is even,} \\ \log n, & \text{if } n \text{ is odd.} \end{cases}$$

Then:

$$\begin{aligned} \text{If } n \text{ is even: } f(n) &= \log n, \quad g(n) = n, \quad \frac{f(n)}{g(n)} = \frac{\log n}{n} \rightarrow 0, \\ \text{If } n \text{ is odd: } f(n) &= n + \log n, \quad g(n) = \log n, \quad \frac{f(n)}{g(n)} \sim \frac{n}{\log n} \rightarrow \infty. \end{aligned}$$

Question assigned to the following page: [2.3](#)



Thus, there is no constant  $C$  such that  $f(n) \leq C g(n)$  for all large  $n$  (so  $f(n) \notin O(g(n))$ ). However,  $f(n)$  also does not satisfy the definition of  $\omega(g(n))$  because for even  $n$ ,  $\lim_{n \rightarrow \infty} f(n)/g(n)$  is 0 but not  $\infty$ .



Problem 3 (20 pts)

Let  $f(n)$  and  $g(n)$  be non-negative functions.

(a) Using the formal definition of  $\Theta()$ , prove that  $\max(f(n), g(n)) = \Theta(f(n) + g(n))$ , where

$$\max(a, b) = \begin{cases} a & \text{if } a \geq b \\ b & \text{otherwise} \end{cases}.$$

(b) Can we also show that  $\min(f(n), g(n)) = \Theta(f(n) + g(n))$ , where

$$\min(a, b) = \begin{cases} a & \text{if } a \leq b \\ b & \text{otherwise} \end{cases}?$$

If yes, show how the proof from part (a) needs to be adapted. If no, provide a counter-example.

## Solution

(a)

Since both  $f(n)$  and  $g(n)$  are nonnegative,

$$\max(f(n), g(n)) = \begin{cases} f(n), & \text{if } f(n) \geq g(n) \\ g(n), & \text{otherwise} \end{cases}.$$

In either case,

$$f(n) \leq \max(f(n), g(n)) \quad \text{and} \quad g(n) \leq \max(f(n), g(n)).$$

Adding these two inequalities we have:

$$f(n) + g(n) \leq 2 \max(f(n), g(n)) \implies \max(f(n), g(n)) \geq \frac{1}{2}(f(n) + g(n)).$$

Also, clearly,

$$\max(f(n), g(n)) \leq f(n) + g(n).$$

Thus, we have

$$\frac{1}{2}(f(n) + g(n)) \leq \max(f(n), g(n)) \leq f(n) + g(n).$$

This shows

$$\max(f(n), g(n)) = \Theta(f(n) + g(n)),$$

with constants  $c_1 = \frac{1}{2}$  and  $c_2 = 1$ .

(b)

It is always true that

$$\min(f(n), g(n)) \leq f(n) + g(n),$$

however, for the equality  $\min(f(n), g(n)) = \Theta(f(n) + g(n))$  to hold we would also require a constant  $c > 0$  such that

$$\min(f(n), g(n)) \geq c(f(n) + g(n))$$

Question assigned to the following page: [3.2](#)

for all sufficiently large  $n$ . We will show a counterexample.

Counterexample: Let

$$f(n) = n \quad \text{and} \quad g(n) = 1 \quad \text{for all } n.$$

Then,

$$\min(f(n), g(n)) = \min(n, 1) = 1,$$

and

$$f(n) + g(n) = n + 1.$$

Given  $\min(f(n), g(n)) = \Theta(f(n) + g(n))$ , there exist constants  $c_1, c_2 > 0$  and  $n_0$  such that for all  $n \geq n_0$ ,

$$c_1(n + 1) \leq 1 \leq c_2(n + 1).$$

While the upper bound  $1 \leq c_2(n + 1)$  holds for any  $c_2 \geq 0$  and large  $n$ , the lower bound

$$1 \geq c_1(n + 1)$$

cannot hold for any fixed  $c_1 > 0$  as  $n \rightarrow \infty$ . Thus, the equality does not hold in general and we cannot say that

$$\min(f(n), g(n)) = \Theta(f(n) + g(n)).$$

Question assigned to the following page: [4.1](#)

Problem 4 (30 pts)

You are given the coefficients  $\alpha_0, \alpha_1, \dots, \alpha_n$  of a polynomial

$$\begin{aligned} P(x) &= \sum_{k=0}^n \alpha_k x^k \\ &= \alpha_0 + \alpha_1 x + \alpha_2 x^2 + \dots + \alpha_n x^n, \end{aligned}$$

and you want to evaluate this polynomial for a given value of  $x$ . *Horner's rule* says to evaluate the polynomial according to this parenthesization:

$$P(x) = \alpha_0 + x \left( \alpha_1 + x \left( \alpha_2 + \dots + x (\alpha_{n-1} + x \alpha_n) \dots \right) \right).$$

The procedure HORNER implements Horner's rule to evaluate  $P(x)$ , give the coefficients  $\alpha_0, \alpha_1, \dots, \alpha_n$  in an array  $A[0 : n]$  and the value of  $x$ .

---

HORNER( $A, n, x$ )

```
1:  $p \leftarrow 0$ 
2: for  $i = n$  to 0 do
3:    $p \leftarrow A[i] + x \cdot p$ 
4: end for
5: return  $p$ 
```

---

For this problem, assume that addition and multiplication can be done in constant time.

- (a) In terms of  $\Theta$ -notation, what is the running time of this procedure?
- (b) Write pseudocode to implement the naive polynomial-evaluation algorithm that computes each term of the polynomial from scratch. What is the running time of this algorithm? How does it compare to HORNER?
- (c) Consider the following loop invariant for the procedure HORNER:  
At the start of each iteration of the **for** loop of lines 2-3,

$$p = \sum_{k=0}^{n-(i+1)} A[k+i+1] \cdot x^k.$$

Interpret a summation with no terms as equaling 0. Following the structure of the loop-invariant proof presented in class, use this loop invariant to show that, at termination,  $p = \sum_{k=0}^n A[k] \cdot x^k$ .

## Solution

(a)

The for loop in HORNER iterates from  $i = n$  down to 0, i.e., it makes  $n + 1$  iterations. In each iteration, a constant number of operations is performed (one multiplication and one addition).

Questions assigned to the following page: [4.2](#), [4.3](#), and [4.1](#)



Thus, the total running time is proportional to  $n + 1$ . In  $\Theta$ -notation we have:

$$T(n) = \Theta(n).$$

(b)

A naive method to evaluate

$$P(x) = \sum_{k=0}^n A[k] x^k$$

is to compute each term  $A[k] \cdot x^k$  from scratch and sum them.

NAIVEPOLYEVAL( $A, n, x$ ):

```
1:  $p \leftarrow 0$ 
2: for  $k = 0$  to  $n$  do
3:    $term \leftarrow 1$ 
4:   for  $j = 1$  to  $k$  do
5:      $term \leftarrow term \cdot x$ 
6:   end for
7:    $p \leftarrow p + A[k] \cdot term$ 
8: end for
9: return  $p$ 
```

In this algorithm, for each  $k$  the inner loop runs  $k$  times. Therefore, the total number of multiplications is

$$\sum_{k=0}^n k = \frac{n(n+1)}{2} = \Theta(n^2).$$

Thus, the running time of the naive algorithm is  $\Theta(n^2)$ , which is asymptotically slower than Horner's  $\Theta(n)$  method.

(c)

We consider the following loop invariant:

At the start of each iteration of the for-loop (lines 2–3),  $p = \sum_{k=0}^{n-(i+1)} A[k+i+1] \cdot x^k$ .

We want to show that when the loop terminates,  $p = \sum_{k=0}^n A[k] \cdot x^k$ .

**Initialization:**

When the loop begins,  $i = n$ . Then the invariant claims that:

$$p = \sum_{k=0}^{n-(n+1)} A[k+n+1] \cdot x^k.$$

Since the upper limit is  $n - (n + 1) = -1$ , the summation is empty and by convention equals 0. This matches the initialization  $p \leftarrow 0$ , so the invariant holds initially.

**Maintenance:**

Suppose the invariant holds at the start of an iteration for some index  $i$ , so that:

$$p = \sum_{k=0}^{n-(i+1)} A[k+i+1] \cdot x^k.$$

Question assigned to the following page: [4.3](#)

In the body of the loop, we update  $p$  as follows:

$$p \leftarrow A[i] + x \cdot p.$$

Substituting the invariant expression into this update gives:

$$p = A[i] + x \left( \sum_{k=0}^{n-(i+1)} A[k+i+1] \cdot x^k \right) = A[i] + \sum_{k=0}^{n-(i+1)} A[k+i+1] \cdot x^{k+1}.$$

Reindex the summation by letting  $j = k + 1$ . Then when  $k = 0$ ,  $j = 1$ , and when  $k = n - (i + 1)$ ,  $j = n - i$ . This gives:

$$p = A[i] + \sum_{j=1}^{n-i} A[j+i] \cdot x^j = \sum_{j=0}^{n-i} A[j+i] \cdot x^j,$$

where we have written  $A[i]$  as the term corresponding to  $j = 0$ . This is exactly the loop invariant for the next iteration (with  $i$  replaced by  $i - 1$ ).

**Termination:**

The loop terminates when  $i = -1$ . At this point, the invariant gives:

$$p = \sum_{k=0}^{n-((-1)+1)} A[k+(-1)+1] \cdot x^k = \sum_{k=0}^n A[k] \cdot x^k.$$

Hence, upon termination,  $p = P(x)$ .

This completes the loop invariant proof that HORNER correctly evaluates the polynomial.

No questions assigned to the following page.

